theories/case_studies/multiuser_kvs/kvs_spec_erase_safe.v
@@ -4,7 +4,7 @@ From griotte Require Import
   switcher kvs kvs_preamble kvs_spec_getFullKey kvs_spec_search kvs_spec_check_uint16.
 From griotte Require Import region_invariants_revocation wp_rules_interp interp_weakening.
 From griotte Require Import switcher_preamble switcher_spec_return.
-From griotte Require Import proofmode map_simpl.
+From griotte Require Import proofmode map_simpl register_tactics.
 
 Section KVS_spec_erase.
   Context
@@ -45,13 +45,14 @@ Section KVS_spec_erase.
       ca1 ↦ᵣ wca1 ∗ (* Key to erase *)
       ct1 ↦ᵣ - ∗ (* scratch *)
       ct2 ↦ᵣ - ∗ (* scratch *)
+      ctp ↦ᵣ - ∗ (* scratch *)
       cnull ↦ᵣ - ∗
 
       (* initial memory layout *)
       codefrag pc_a kvs_erase_instrs ∗
-      cgp_b ↦ₐ kvs_service_unsealing_key ∗
+      (pc_b ^+ UNSEALING_USER_KEY_OFFSET)%a ↦ₐ kvs_service_unsealing_key ∗
 
-      ▷ isKVS (cgp_b ^+ 1)%a m s ∗
+      ▷ isKVS cgp_b m s ∗
       ▷ seal_pred KVS_OTYPE kvs_otype_propC ∗
 
       world_interp W C ∗
@@ -64,16 +65,17 @@ Section KVS_spec_erase.
          ca1 ↦ᵣ WInt 0 ∗
          ct1 ↦ᵣ - ∗ (* scratch *)
          ct2 ↦ᵣ - ∗ (* scratch *)
+         ctp ↦ᵣ - ∗ (* scratch *)
          cnull ↦ᵣ - ∗
 
          codefrag pc_a kvs_erase_instrs ∗
-         cgp_b ↦ₐ kvs_service_unsealing_key ∗
+         (pc_b ^+ UNSEALING_USER_KEY_OFFSET)%a ↦ₐ kvs_service_unsealing_key ∗
 
          (
            (∃ idx ku kn,
-             isKVS (cgp_b ^+ 1)%a (<[ idx := (EMPTY_SLOT, WInt DEFAULT_VAL) ]> m) (kvs_alloc_delete s ku {[kn]}))
+             isKVS cgp_b (<[ idx := (EMPTY_SLOT, WInt DEFAULT_VAL) ]> m) (kvs_alloc_delete s ku {[kn]}))
          ∨
-             (isKVS (cgp_b ^+ 1)%a m s)
+             (isKVS cgp_b m s)
          ) ∗
 
          world_interp W C
@@ -83,15 +85,15 @@ Section KVS_spec_erase.
       ⊢ WP Seq (Instr Executable) {{ v, ⌜v = HaltedV⌝ → na_own cerise_nais ⊤ }})%I.
   Proof.
     iIntros (HN HsubBounds Hcgp_contiguous Hrelated_Wca0_W)
-      "(Hna & HPC & Hcgp & Hcra & Hca0 & Hinterp_wca0 & Hca1 & Hct1 & Hct2 & [%wcnull Hcnull] &
-        Hcode & Hcgp_b & HKVS & #Hspred & Hworld & Hpost)".
+      "(Hna & HPC & Hcgp & Hcra & Hca0 & Hinterp_wca0 & Hca1 & Hct1 & Hct2 & Hctp & [%wcnull Hcnull] &
+        Hcode & Ha_unsealing & HKVS & #Hspred & Hworld & Hpost)".
     codefrag_facts "Hcode"; rename H into Hpc_contiguous ; clear H0.
 
     (* --------------------------------------------------- *)
     (* ----------------- Start the proof ----------------- *)
     (* --------------------------------------------------- *)
     rewrite /kvs_erase_instrs /assembled_kvs_erase.
-    rewrite -/(kvs_getFullKey ca0 ca0 ca1 ct1).
+    rewrite -/(kvs_getFullKey ctp ca0 ca1 ct1 ct2).
     rewrite -/(kvs_search ca0 ct1 ct2).
     rewrite -/(kvs_check_uint16 ca1 ct1).
 
@@ -124,16 +126,14 @@ Section KVS_spec_erase.
     focus_block 2 "Hcode" as a_get_full_key Ha_get_full_key "Hcode" "Hcont"; iHide "Hcont" as hcont
     ; clear dependent Ha_check_uint.
     iApply (KVS_getFullKey_spec_safe with
-             "[- $HPC $Hcgp $Hca0 $Hinterp_wca0 $Hca1 $Hct1 $Hcgp_b $Hcode $Hspred $Hworld]")
-    ; eauto; [|iNext].
-    { rewrite /withinBounds; solve_addr. }
+             "[- $HPC $Hctp $Hca0 $Hinterp_wca0 $Hca1 $Hct1 $Hct2 $Ha_unsealing $Hcode $Hspred $Hworld]")
+    ; eauto; iNext.
     iIntros (l_user_key user_key)
-      "([%Huser_key_C ->] & HPC & Hcgp & Hca0 & Hca1 & Hct1 & Hcgp_b & Hcode & #Hseal_ku & Hworld)".
+      "([%Huser_key_C ->] & HPC & Hctp & Hca0 & Hca1 & Hct1 & Hct2 & Ha_unsealing & Hcode & #Hseal_ku & Hworld)".
     subst hcont; unfocus_block "Hcode" "Hcont" as "Hcode".
 
     focus_block 3 "Hcode" as a_lea Ha_lea "Hcode" "Hcont"; iHide "Hcont" as hcont ; clear dependent Ha_get_full_key.
     iInstr "Hcode" with "Hlc".
-    { transitivity (Some (cgp_b ^+ 1)%a); [solve_addr|done]. }
     subst hcont; unfocus_block "Hcode" "Hcont" as "Hcode".
 
     focus_block 4 "Hcode" as a_search Ha_search "Hcode" "Hcont"; iHide "Hcont" as hcont; clear dependent Ha_lea.
@@ -174,7 +174,7 @@ Section KVS_spec_erase.
       { solve_addr+Hcgp_idx. }
       (* Lea cgp 1 *)
       iInstr "Hcode".
-      { transitivity ( Some ((cgp_b ^+ (2 + 2 * idx))%a) ); solve_addr+Hcgp_idx Hidx. }
+      { transitivity ( Some ((cgp_b ^+ (2 * idx + 1))%a) ); solve_addr+Hcgp_idx Hidx. }
       (* Store cgp (inr ca2) *)
       iInstr_lookup "Hcode" as "Hi" "Hcode".
       wp_instr.
@@ -197,8 +197,8 @@ Section KVS_spec_erase.
       iDestruct (close_isKVS with "[$HKVS Hcgp_key Hcgp_val Hkvs_frag]") as "HKVS";eauto.
       { by simplify_map_eq. }
       {
-        replace (cgp_b ^+ (1 + 2 * idx))%a with ((cgp_b ^+ 1) ^+ 2 * idx)%a by solve_addr+Hidx.
-        replace (cgp_b ^+ (2 + 2 * idx))%a  with ((cgp_b ^+ 1) ^+ (2 * idx + 1))%a by solve_addr+Hidx.
+        replace (cgp_b ^+ (2 * idx ))%a with (cgp_b ^+ 2 * idx)%a by solve_addr+Hidx.
+        replace (cgp_b ^+ (2 * idx + 1))%a  with (cgp_b ^+ (2 * idx + 1))%a by solve_addr+Hidx.
         iFrame.
       }
 
@@ -262,6 +262,7 @@ Section KVS_spec_erase.
       ca1 ↦ᵣ wca1 ∗ (* Key to update *)
       ct1 ↦ᵣ - ∗ (* scratch *)
       ct2 ↦ᵣ - ∗ (* scratch *)
+      ctp ↦ᵣ - ∗ (* scratch *)
       cnull ↦ᵣ - ∗
 
       world_interp W C ∗
@@ -274,6 +275,7 @@ Section KVS_spec_erase.
          ca1 ↦ᵣ WInt 0 ∗
          ct1 ↦ᵣ - ∗ (* scratch *)
          ct2 ↦ᵣ - ∗ (* scratch *)
+         ctp ↦ᵣ - ∗ (* scratch *)
          cnull ↦ᵣ - ∗
 
          world_interp W C
@@ -284,15 +286,21 @@ Section KVS_spec_erase.
   Proof.
     iIntros (Hnkvs_E Hnkvs_otype_E Hrelated_Wca0_W)
       "(#Hkvs_inv & Hna & HPC & Hcgp & Hcra & Hca0 & Hinterp_ca0
-      & Hca1 & Hct1 & Hct2 & Hcnull & Hworld & Hpost)".
+      & Hca1 & Hct1 & Hct2 & Hctp & Hcnull & Hworld & Hpost)".
     iMod (na_inv_acc with "Hkvs_inv Hna")
-      as "( (%m & %s & >Himports & >Hcode & >Hcgp_b & HisKVS & #Hspred) & Hna & Hkvs_inv_close)"; eauto.
+      as "( (%m & %s & >Himports & >Hcode & HisKVS & #Hspred) & Hna & Hkvs_inv_close)"; eauto.
     pose proof (Hcgp_continuous := KVS_size_data).
     pose proof (HKVS_pcc_b' := KVS_size_imports).
     pose proof (Hcode_continuous := KVS_size_code).
     assert (SubBounds KVS_pcc_b KVS_pcc_e kvs_erase_pcc_addr (kvs_erase_pcc_addr ^+ length kvs_erase_instrs)%a) as HSubBounds.
     { rewrite /kvs_erase_pcc_addr; cbn in *; solve_addr. }
     codefrag_facts "Hcode"; rename H into Hpc_contiguous.
+    rewrite /kvs_imports /kvs.kvs_imports_pre.
+    assert ((KVS_pcc_b + 1)%a = Some (KVS_pcc_b ^+ 1)%a) by ( rewrite /length_kvs_imports in HKVS_pcc_b'; solve_addr+ HKVS_pcc_b').
+    assert ((KVS_pcc_b ^+ 1)%a <= KVS_pcc_b')%a  by ( rewrite /length_kvs_imports in HKVS_pcc_b'; solve_addr+ HKVS_pcc_b').
+    assert ((KVS_pcc_b ^+ 1 + 1)%a = Some (KVS_pcc_b')%a) by ( rewrite /length_kvs_imports in HKVS_pcc_b'; solve_addr+ HKVS_pcc_b').
+    iDestruct (region_pointsto_cons with "Himports") as "[Himports_sw Himports]"; eauto.
+    iDestruct (region_pointsto_single with "Himports") as "(% & Ha_unsealing & %Heq)"; eauto; simplify_eq.
 
     rewrite /kvs_service_instrs.
     focus_block_nochangePC 2 "Hcode" as a_erase Ha_erase "Hcode" "Hcont"; iHide "Hcont" as hcont.
@@ -300,13 +308,16 @@ Section KVS_spec_erase.
       as -> by (rewrite /kvs_erase_pcc_addr ; cbn in * ; solve_addr+Hcode_continuous HKVS_pcc_b' Ha_erase).
     iApply (KVS_erase_spec_safe_pre with "[- $HPC]"); last iFrame "∗#"; eauto.
     { pose proof Nkvs_namespaces_disjoint as (?&?&?); solve_ndisj. }
-    iNext; iIntros "(Hna & HPC & Hcgp & Hcra & Hca0 & Hca1 & Hct1 & Hct2 & Hcnull
-     & Hcode & Hcgp_b & HKVS & Hworld)".
+    iNext; iIntros "(Hna & HPC & Hcgp & Hcra & Hca0 & Hca1 & Hct1 & Hct2 & Hctp & Hcnull
+     & Hcode & Ha_unsealing & HKVS & Hworld)".
     subst hcont; unfocus_block "Hcode" "Hcont" as "Hcode".
 
     iDestruct "HKVS" as "[ (%idx & %ku & %kn & HKVS) | HKVS ]".
-    all: iMod ("Hkvs_inv_close" with "[$Hna $Himports $Hcode $Hcgp_b $HKVS $Hspred]") as "Hna".
-    all: iApply "Hpost"; iFrame.
+    all: iMod ("Hkvs_inv_close" with "[$Hna Himports_sw $Hcode Ha_unsealing $HKVS $Hspred]") as "Hna" ; last (iApply "Hpost"; iFrame).
+    all: iNext.
+    all: iApply (region_pointsto_cons with "[Ha_unsealing Himports_sw]"); eauto; iFrame.
+    all: iApply (region_pointsto_cons with "[Ha_unsealing]"); eauto; [solve_addr+|]; iFrame.
+    all: rewrite /region_pointsto finz_seq_between_empty; auto; solve_addr+.
   Qed.
 
 
@@ -357,27 +368,14 @@ Section KVS_spec_erase.
     rewrite /registers_pointsto.
 
     (* Extract the registers that we will need *)
-    iDestruct (big_sepM_delete _ _ PC with "Hrmap") as "[HPC Hrmap]"; first by simplify_map_eq.
-    iDestruct (big_sepM_delete _ _ cgp with "Hrmap") as "[Hcgp Hrmap]"; first by simplify_map_eq.
-    iDestruct (big_sepM_delete _ _ cra with "Hrmap") as "[Hcra Hrmap]"; first by simplify_map_eq.
-    iDestruct (big_sepM_delete _ _ csp with "Hrmap") as "[Hcsp Hrmap]"; first by simplify_map_eq.
-    (* General purpose registers *)
-    assert ( is_Some (rmap !! ct1) ) as [wct1 Hwct1].
-    { apply Hrmap_init; rewrite Hrmap_dom ; done. }
-    iDestruct (big_sepM_delete _ _ ct1 with "Hrmap") as "[Hct1 Hrmap]"; first by simplify_map_eq.
-    assert ( is_Some (rmap !! ct2) ) as [wct2 Hwct2].
-    { apply Hrmap_init; rewrite Hrmap_dom ; done. }
-    iDestruct (big_sepM_delete _ _ ct2 with "Hrmap") as "[Hct2 Hrmap]"; first by simplify_map_eq.
-    assert ( is_Some (rmap !! cnull) ) as [wcnull Hwcnull].
-    { apply Hrmap_init; rewrite Hrmap_dom ; done. }
-    iDestruct (big_sepM_delete _ _ cnull with "Hrmap") as "[Hcnull Hrmap]"; first by simplify_map_eq.
-    (* Argument registers *)
-    assert ( is_Some (rmap !! ca0) ) as [wca0 Hwca0].
-    { apply Hrmap_init; rewrite Hrmap_dom ; done. }
-    iDestruct (big_sepM_delete _ _ ca0 with "Hrmap") as "[Hca0 Hrmap]"; first by simplify_map_eq.
-    assert ( is_Some (rmap !! ca1) ) as [wca1 Hwca1].
-    { apply Hrmap_init; rewrite Hrmap_dom ; done. }
-    iDestruct (big_sepM_delete _ _ ca1 with "Hrmap") as "[Hca1 Hrmap]"; first by simplify_map_eq.
+    assert ( is_Some (rmap !! ctp) ) as [wctp Hwctp] by ( apply Hrmap_init; rewrite Hrmap_dom ; done ).
+    assert ( is_Some (rmap !! ct1) ) as [wct1 Hwct1] by ( apply Hrmap_init; rewrite Hrmap_dom ; done ).
+    assert ( is_Some (rmap !! ct2) ) as [wct2 Hwct2] by ( apply Hrmap_init; rewrite Hrmap_dom ; done ).
+    assert ( is_Some (rmap !! ca0) ) as [wca0 Hwca0] by ( apply Hrmap_init; rewrite Hrmap_dom ; done ).
+    assert ( is_Some (rmap !! ca1) ) as [wca1 Hwca1] by ( apply Hrmap_init; rewrite Hrmap_dom ; done ).
+    assert ( is_Some (rmap !! cnull) ) as [wcnull Hwcnull] by ( apply Hrmap_init; rewrite Hrmap_dom ; done ).
+    iExtractList "Hrmap" [PC; cgp; cra ; csp ] as ["HPC"; "Hcgp"; "Hcra"; "Hcsp"].
+    iExtractList "Hrmap" [ct1; ct2; ctp; cnull; ca0; ca1] as ["Hct1"; "Hct2"; "Hctp"; "Hcnull"; "Hca0"; "Hca1"].
 
     iAssert (interp W0 C wca0) as "#Hinterp_wca0".
     { iApply "Hinterp_rmap"; eauto; by rewrite /kvs_erase_nargs. }
@@ -393,15 +391,16 @@ Section KVS_spec_erase.
     assert (related_sts_priv_world W0 W1) as Hrelared_priv_W0_W1 by eapply revoke_related_sts_priv_world.
 
     iApply (KVS_erase_spec_safe W0 (revoke W0)); try solve_ndisj; iFrame "#∗".
-    iNext; iIntros "(Hna & HPC & Hcgp & Hcra & Hca0 & Hca1 & Hct1 & Hct2 & Hcnull & Hworld_C)".
+    iNext; iIntros "(Hna & HPC & Hcgp & Hcra & Hca0 & Hca1 & Hct1 & Hct2 & Hctp & Hcnull & Hworld_C)".
     set (Wfixed := (close_list (l ++ finz.seq_between csp_b csp_e) (revoke W0))).
     iAssert (∃ wca0', ca0 ↦ᵣ wca0' ∗ interp Wfixed C wca0')%I with "[Hca0]" as "(%wca0' & Hca0 & #Hinterp_wca0')".
     { iDestruct "Hca0" as "[$|$]"; iApply interp_int. }
     iAssert (∃ wca1', ca1 ↦ᵣ wca1' ∗ interp Wfixed C wca1')%I with "[Hca1]" as "(%wca1' & Hca1 & #Hinterp_wca1')".
     { iFrame "Hca1"; iApply interp_int. }
 
-
     iDestruct "Hcnull" as "[% Hcnull]"; iDestruct (big_sepM_insert _ _ cnull with "[$Hrmap $Hcnull]") as "Hrmap".
+    { repeat (rewrite lookup_insert_ne; auto); apply not_elem_of_dom_1; set_solver+. }
+    iDestruct "Hctp" as "[% Hctp]"; iDestruct (big_sepM_insert _ _ ctp with "[$Hrmap $Hctp]") as "Hrmap".
     { repeat (rewrite lookup_insert_ne; auto); apply not_elem_of_dom_1; set_solver+. }
     iDestruct "Hct2" as "[% Hct2]"; iDestruct (big_sepM_insert _ _ ct2 with "[$Hrmap $Hct2]") as "Hrmap".
     { repeat (rewrite lookup_insert_ne; auto); apply not_elem_of_dom_1; set_solver+. }
@@ -423,6 +422,7 @@ Section KVS_spec_erase.
     { apply regmap_full_dom in Hrmap_init.
       repeat (rewrite dom_insert_L).
       repeat (rewrite dom_delete_L).
+      repeat (rewrite dom_insert_L).
       rewrite Hrmap_init. set_solver+. }
     { subst csp_b. destruct Hsync_csp as [Hsync_csp <-]; eauto. }
     { intros a Ha; apply Htemps; done. }
